Change import order of Atom and FunctionFreeAtom

ExistentialRules/AtomsAndRules/Atom.lean
@@ -6,7 +6,7 @@ Released under Apache 2.0 license as described in the file LICENSE.
 module
 
 public import ExistentialRules.Terms.SkolemTerm
-public import ExistentialRules.AtomsAndRules.Basic
+public import ExistentialRules.AtomsAndRules.FunctionFreeAtom
 
 /-!
 # Atom
@@ -17,4 +17,33 @@ An `Atom` is simply a `GeneralizedAtom` using `SkolemTerm`s.
 public section
 
 abbrev Atom (sig : Signature) [DecidableEq sig.P] [DecidableEq sig.C] [DecidableEq sig.V] := GeneralizedAtom sig (SkolemTerm sig)
+
+namespace FunctionFreeAtom
+
+variable {sig : Signature} [DecidableEq sig.P] [DecidableEq sig.C] [DecidableEq sig.V]
+
+/-- We can `skolemize` a `FunctionFreeAtom` by skolemizing all its `VarOrConst`s. This yields an `Atom`. -/
+def skolemize (ruleId : Nat) (disjunctIndex : Nat) (frontier : List sig.V) (a : FunctionFreeAtom sig) : Atom sig := {
+  predicate := a.predicate,
+  terms := a.terms.map (VarOrConst.skolemize ruleId disjunctIndex frontier),
+  arity_ok := by rw [List.length_map, a.arity_ok]
+}
+
+/-- The number of terms remains unchanged when Skolemizing. -/
+@[simp, grind =]
+theorem length_skolemize {ruleId : Nat} {disjunctIndex : Nat} {frontier : List sig.V} {a : FunctionFreeAtom sig} :
+    (a.skolemize ruleId disjunctIndex frontier).terms.length = a.terms.length := by
+  unfold skolemize; simp
+
+/-- If a a `VarOrConst` occurs in the terms of the `FunctionFreeAtom`, then the Skolemized `VarOrConst` occurs in the Skolemized `Atom`. -/
+@[grind <-]
+theorem mem_skolemize_of_mem {ruleId : Nat} {disjunctIndex : Nat} {frontier : List sig.V}
+    {a : FunctionFreeAtom sig} {t : VarOrConst sig} :
+    t ∈ a.terms -> (t.skolemize ruleId disjunctIndex frontier) ∈ (a.skolemize ruleId disjunctIndex frontier).terms := by
+  unfold skolemize
+  intro t_mem
+  rw [List.mem_map]
+  exists t
+
+end FunctionFreeAtom
 
