ExistentialRules/AtomsAndRules/FunctionFreeAtom.lean
@@ -5,7 +5,7 @@ Released under Apache 2.0 license as described in the file LICENSE.
 
 module
 
-public import ExistentialRules.AtomsAndRules.Atom
+public import ExistentialRules.AtomsAndRules.Basic
 
 /-!
 # FunctionFreeAtom
@@ -29,13 +29,6 @@ def variables (a : FunctionFreeAtom sig) : List sig.V := VarOrConst.filterVars a
 @[expose]
 def constants (a : FunctionFreeAtom sig) : List sig.C := VarOrConst.filterConsts a.terms
 
-/-- We can `skolemize` a `FunctionFreeAtom` by skolemizing all its `VarOrConst`s. This yields an `Atom`. -/
-def skolemize (ruleId : Nat) (disjunctIndex : Nat) (frontier : List sig.V) (a : FunctionFreeAtom sig) : Atom sig := {
-  predicate := a.predicate,
-  terms := a.terms.map (VarOrConst.skolemize ruleId disjunctIndex frontier),
-  arity_ok := by rw [List.length_map, a.arity_ok]
-}
-
 /-- A variable occurs in `variables` iff it is a term of the `FunctionFreeAtom. -/
 @[simp, grind =]
 theorem mem_variables {a : FunctionFreeAtom sig} {v : sig.V} : v ∈ a.variables ↔ (VarOrConst.var v) ∈ a.terms := by
@@ -45,22 +38,6 @@ theorem mem_variables {a : FunctionFreeAtom sig} {v : sig.V} : v ∈ a.variables
 @[simp, grind =]
 theorem mem_constants {a : FunctionFreeAtom sig} {c : sig.C} : c ∈ a.constants ↔ (VarOrConst.const c) ∈ a.terms := by
   unfold constants; grind
-
-/-- The number of terms remains unchanged when Skolemizing. -/
-@[simp, grind =]
-theorem length_skolemize {ruleId : Nat} {disjunctIndex : Nat} {frontier : List sig.V} {a : FunctionFreeAtom sig} :
-    (a.skolemize ruleId disjunctIndex frontier).terms.length = a.terms.length := by
-  unfold skolemize; simp
-
-/-- If a a `VarOrConst` occurs in the terms of the `FunctionFreeAtom`, then the Skolemized `VarOrConst` occurs in the Skolemized `Atom`. -/
-@[grind <-]
-theorem mem_skolemize_of_mem {ruleId : Nat} {disjunctIndex : Nat} {frontier : List sig.V}
-    {a : FunctionFreeAtom sig} {t : VarOrConst sig} :
-    t ∈ a.terms -> (t.skolemize ruleId disjunctIndex frontier) ∈ (a.skolemize ruleId disjunctIndex frontier).terms := by
-  unfold skolemize
-  intro t_mem
-  rw [List.mem_map]
-  exists t
 
 end FunctionFreeAtom
 
